Classes/SoundMonad.v
@@ -1,0 +1,26 @@
+Require Export Base.
+Require Import Classes.PreorderedSet.
+Require Import Classes.Galois.
+Require Import Classes.Functor.
+Require Import Classes.Applicative.
+Require Import Classes.Monad.
+Require Import Instances.Galois.
+
+Section sound_monad.
+  Context (M M' : Type → Type) `{Monad M, Monad M'}.
+  Context {M_preorder : ∀ T', PreorderedSet T' → PreorderedSet (M' T')}.
+  Context {M_galois : ∀ T T' {HT : PreorderedSet T'}, Galois T T' → Galois (M T) (M' T')}.
+
+  Class SoundMonad : Type :=
+  {
+    fmap_sound : ∀ (A A' B B' : Type ) `{Galois A A', Galois B B'},
+      gamma (fmap (F:=M') (A:=A') (B:=B')) (fmap (F:=M) (A:=A) (B:=B));
+    pure_sound : ∀ (A A' : Type) `{Galois A A'},
+      gamma (pure (F:=M') (A:=A')) (pure (F:=M) (A:=A));
+    app_sound : ∀ (A A' B B' : Type) `{Galois A A', Galois B B'},
+      gamma (app (F:=M') (A:=A') (B:=B')) (app (F:=M) (A:=A) (B:=B));
+    bind_sound : ∀ (A A' B B' : Type) `{Galois A A', Galois B B'},
+      gamma (bindM (M:=M') (A:=A') (B:=B')) (bindM (M:=M) (A:=A) (B:=B));
+  }.
+End sound_monad.
+Hint Resolve fmap_sound pure_sound app_sound bind_sound : soundness.
